
\begin{exercises}

	\begin{problist}
		\prob
		\begin{enumerate}
			\item Let $\mathcal U:\R^{2}\to\R^{2}$ be the matrix transformation
				given by $\mat{0&0\\-\sqrt{2}/2 & -\sqrt{2}/2}$. Further,
				let $\mathcal P:\R^{2}\to\R^{2}$ be the projection onto
				the $y$-axis, and let $\mathcal R:\R^{2}\to\R^{2}$ be the rotation
				clockwise by $135^{\circ}$.
				\begin{enumerate}
					\item Find a matrix for $\mathcal R \circ \mathcal
						P$.

					\item Find a matrix for $\mathcal P \circ \mathcal
						R$.

					\item Write $\mathcal U$ as the composition (in some
						order) of $\mathcal R$ and $\mathcal P$.
				\end{enumerate}

			\item Let $\mathcal V:\R^{2}\to\R^{2}$ be the matrix transformation
				given by $\mat{0&2\\2&0}$. Further, let
				$\mathcal S:\R^{2}\to\R^{2}$ be the transformation that
				doubles every vector, and let $\mathcal F:\R^{2}\to\R^{2}$
				be the transformation reflecting over the line $y=x$.
				\begin{enumerate}
					\item Find a matrix for $\mathcal F \circ \mathcal
						S$.

					\item Find a matrix for $\mathcal S \circ \mathcal
						F$.

					\item Write $\mathcal V$ as the composition (in some
						order) of $\mathcal F$ and $\mathcal S$.
				\end{enumerate}
		\end{enumerate}

		% Q1 Solutions

		\begin{solution}

			\begin{enumerate}
				\item $(\mathcal R \circ \mathcal P)(\mat{1\\0}) = \mat{0\\0}$,
					$(\mathcal R \circ \mathcal P)(\mat{0\\1}) = \mat{\tfrac{1}{\sqrt{2}}\\
					-\tfrac{1}{\sqrt{2}}}$, $(\mathcal P \circ \mathcal
					R)(\mat{1\\0}) = \mat{0\\ -\tfrac{1}{\sqrt{2}}}$,
					$(\mathcal P \circ \mathcal R)(\mat{0\\1}) = \mat{0\\
					- \tfrac{1}{\sqrt{2}}}$. We can use the effect of the
					transformation on the standard basis to compute the
					matrix.


					\begin{enumerate}
						\item $M_{R\circ P}= \mat{\mathcal R(\mathcal
							P(\xhat))& \mathcal R( \mathcal P(\yhat))}=
							\mat{0&\tfrac{1}{\sqrt{2}}\\0&-\tfrac{1}{\sqrt{2}}}$

						\item $M_{P\circ R}= \mat{\mathcal P(
							\mathcal R(\xhat))& \mathcal P(\mathcal
							R(\yhat))}= \mat{0&0\\-\tfrac{1}{\sqrt{2}}&-\tfrac{1}{\sqrt{2}}}$

						\item Since $M_{\mathcal U}=M_{\mathcal P
							\circ \mathcal R}$ and $\tfrac{1}{\sqrt{2}}=\tfrac{\sqrt{2}}{2}$,
							we can assert that
							$\mathcal U=\mathcal P \circ
							\mathcal R$.
					\end{enumerate}

				\item $(\mathcal F \circ \mathcal S)(\mat{1\\0}) = \mat{0\\2}$,
					$(\mathcal F \circ \mathcal S)(\mat{0\\1}) = \mat{2\\0}$,
					$(\mathcal S \circ \mathcal F)(\mat{1\\0}) = \mat{0\\2}$,
					$(\mathcal S \circ \mathcal F)(\mat{0\\1}) = \mat{2\\0}$.
					We can use the effect of the transformation on the
					standard basis to compute the matrix.
					\begin{enumerate}
						\item $M_{\mathcal F \circ \mathcal S}=\mat{\mathcal
							F( \mathcal S(\xhat))& \mathcal F(\mathcal
							S(\yhat))}=\mat{0&2\\2&0}$

						\item $M_{\mathcal S \circ \mathcal F}=\mat{\mathcal
							S( \mathcal F(\xhat))& \mathcal S(\mathcal
							F(\yhat))}=\mat{0&2\\2&0}$

						\item $\mathcal S\circ \mathcal F=
							\mathcal V = \mathcal F \circ
							\mathcal S$.
					\end{enumerate}
			\end{enumerate}
		\end{solution}

		\prob Let $\mathcal A: \R^{2}\to \R^{2}$ and
		$\mathcal B: \R^{2}\to \R^{2}$ be matrix transformations with matrices
		\[
			M_{\mathcal A}= \mat{2&2\\1&3}\quad \text{and}\quad M_{\mathcal B}=
			\mat{3&2\\0&4}
		\]
		 and let $M_{\mathcal T}$ be the matrix for
		$\mathcal T=\mathcal A\circ\mathcal B$.
		\begin{enumerate}
			\item Find $M_{\mathcal T}$ by computing input-output pairs for $\mathcal
				T$.

			\item Find $M_{\mathcal T}$ by using matrix multiplication applied
				to $M_{\mathcal A}$ and $M_{\mathcal B}$.
		\end{enumerate}

		% Q2 Solutions

		\begin{solution}

			\begin{enumerate}
				\item $M_{\mathcal T}\mat{1\\0}= M_{\mathcal A}M_{\mathcal
					B}\mat{1\\0}= M_{\mathcal A}\mat{3&2\\0&4}\mat{1\\0}=
					\mat{2&2\\1&3}\mat{3\\0}= \mat{6\\3}$ \\ $M_{\mathcal
					T}\mat{0\\1}= M_{\mathcal A}M_{\mathcal B}\mat{0\\1}=
					M_{\mathcal A}\mat{3&2\\0&4}\mat{0\\1}= \mat{2&2\\1&3}\mat{2\\4}=
					\mat{12\\14}$. Therefore
					$M_{\mathcal T}= \mat{6&12\\3&14}$

				\item $M_{\mathcal T}= M_{\mathcal A}M_{\mathcal B}= \mat{2&2\\1&3}\mat{3&2\\0&4}=
					\mat{6&12\\3&14}$
			\end{enumerate}
		\end{solution}

		\prob Let $\mathcal A: \R^{3}\to \R^{2}$ and $\mathcal B: \R^{2}\to \R^{1}$
		be matrix transformations with matrices
		\[
			M_{\mathcal A}= \mat{2&1&0\\2&3&0}\quad and \quad M_{\mathcal B}=
			\mat{3&2}
		\]
		 and let $M_{\mathcal T}$ be the matrix for $\mathcal T=\mathcal B\circ \mathcal
		A$.
		\begin{enumerate}
			\item Find $M_{\mathcal T}$ by computing input-output pairs for $\mathcal
				T$.

			\item Find $M_{\mathcal T}$ by using matrix multiplication applied
				to $M_{\mathcal A}$ and $M_{\mathcal B}$.
		\end{enumerate}

		% Q3 Solutions

		\begin{solution}

			\begin{enumerate}
				\item $\mathcal T = \mathcal B \circ \mathcal A$, thus
					$\mathcal T : \R^{3}\to \R$. \\ $\mathcal T \mat{1\\0\\0}=
					(\mathcal B \circ \mathcal A) \mat{1\\0\\0}=
					\mathcal B \mat{2\\2}= 10$

					$\mathcal T \mat{0\\1\\0}= (\mathcal B \circ \mathcal
					A) \mat{0\\1\\0}= \mathcal B \mat{1\\3}= 9$

					$\mathcal T \mat{0\\0\\1}= (\mathcal B \circ \mathcal
					A) \mat{0\\0\\1}= \mathcal B \mat{0\\0}= 0$.
					Therefore $M_{\mathcal T}= \mat{10&9&0}$

				\item $M_{\mathcal T}= M_{\mathcal B}M_{\mathcal A}= \mat{3&2}\mat{2&1&0\\2&3&0}=
					\mat{10&9&0}$
			\end{enumerate}
		\end{solution}
	\end{problist}
\end{exercises}
